trying induction n for existsWitnessPath_rtl, stuck

Pdl/Paths.lean
@@ -1,4 +1,3 @@
-
 import Pdl.Unfold
 
 def atomRel {W} (M : KripkeModel W) (v w : W) := ∃ a, relate M (·a) v w
@@ -8,16 +7,86 @@ abbrev WorldPath {W} (M : KripkeModel W) := Subtype $ List.Chain' (atomRel M)
 @[simp]
 def WorldPath.tail (π : WorldPath M) : WorldPath M := ⟨π.1.tail, π.2.tail⟩
 
-/-- Does path `π` starting at v0 witness `¬□(δ,ξ)`? -/
--- NOTE: Not using `WorldPath` any more, atom relation is built in here!
-inductive witness (M : KripkeModel W) : W  → List W → List Program → Formula → Prop
+/-- A path starting at `v0` to witness `¬□(δ,ξ)`. -/
+-- NOTE: Not using `WorldPath` any more, atom relation is built in here.
+inductive witness : KripkeModel W → (v0 : W) → (δ : List Program) → (ξ : Formula) → Type
  -- Case |π| = 0:
-| nil : (M,v0) ⊨ (~ξ) → witness M v0 [] [] ξ
+| nil : evaluate M v0 (~ξ) → witness M v0 [] ξ
  -- Case |π| > 0:
-| consAtom : M.Rel a v0 v1 → witness M v1 rest γs ξ → witness M v0 (v1 :: rest) ((·a) :: γs) ξ
-| consEmpty Fs : (⟨Fs, ε⟩ ∈ H α) → (M, v0) ⊨ Fs → witness M v0 π γs ξ → witness M v0 π (α::γs) ξ
-| consComp : M.Rel a v0 v1 → (⟨Fs, (·a : Program) :: η⟩ ∈ H α) → (M, v0) ⊨ Fs → witness M v1 rest (ηs ++ γs) ξ → witness M v0 (v1 :: rest) (α::γs) ξ
+| consAtom {a} {v1} {γs} :
+    (v0_a_v1 : M.Rel a v0 v1)
+      → witness M v1 γs ξ
+      → witness M v0 ((·a) :: γs) ξ
+| consEmpty Fs :
+    (⟨Fs, ε⟩ ∈ H α)
+      → evaluate M v0 (Con Fs)
+      → witness M v0 γs ξ
+      → witness M v0 (α::γs) ξ
+| consComp :
+    M.Rel a v0 v1
+      → (⟨Fs, (·a : Program) :: ηs⟩ ∈ H α)
+      → evaluate M v0 (Con Fs)
+      → witness M v1 (ηs ++ γs) ξ
+      → witness M v0 (α::γs) ξ
 
+def witness.length : witness M v δ ξ → Nat
+| nil _ => 0
+| consAtom _ wit => 1 + wit.length
+| consEmpty _ _ _ wit => 1 + wit.length
+| consComp _ _ _ wit => 1 + wit.length
+
+theorem existsWitnessPath_rtl (M : KripkeModel W) (n : Nat) :
+    ∀ v δ ξ (wit : witness M v δ ξ),
+      wit.length = n → evaluate M v (~ Formula.boxes δ ξ) := by
+  induction n
+  case zero =>
+    intro v δ ξ wit def_n
+    subst_eqs
+    cases wit
+    case nil =>
+      subst_eqs
+      simp [Formula.boxes, evaluate] at *
+      assumption
+    all_goals
+      exfalso
+      simp [witness.length] at *
+  case succ n IH =>
+    intro v δ ξ wit def_n
+    subst_eqs
+    cases wit
+    case nil =>
+      exfalso
+      subst_eqs
+    case consAtom a v1 γs v0_a_v1 wit_v1_γs =>
+      simp only [evaluate, witness.length, Formula.boxes, relate, not_forall, exists_prop] at *
+      refine ⟨v1, v0_a_v1, IH v1 γs ξ wit_v1_γs ?_⟩
+      linarith
+    case consEmpty α γs Fs Fε_in_Hα v_Fs wit_γs =>
+      simp only [evaluate, witness.length, Formula.boxes, relate, not_forall, exists_prop] at *
+      use v -- no real step
+      constructor
+      · -- need Lemma about H here?
+        sorry
+      · apply IH v γs ξ wit_γs
+        linarith
+    case consComp α Fs v1 ηs γs a Fsaηs_in_Hα v_a_v1 four wit_v1_ηγs =>
+      simp only [evaluate, witness.length, Formula.boxes, relate, not_forall, exists_prop] at *
+      use v1 -- DO a real step here, true??
+      constructor
+      ·
+        -- need Lemma about H here?
+        -- Note α vs a.
+        sorry
+      · specialize IH v1 (ηs++γs) ξ wit_v1_ηγs ?_
+        ·
+          -- PROBLEM: ηs++γs is too long, longer than n. try `induction wit` instead?
+          sorry
+
+        · -- need Lemma about H here?
+          sorry
+
+
+/-
 theorem existsWitnessPath {M : KripkeModel W} δ v :
     (M,v) ⊨ (~ Formula.boxes δ ξ) ↔ ∃ π, witness M v π δ ξ := by
   induction δ generalizing v
@@ -26,9 +95,6 @@ theorem existsWitnessPath {M : KripkeModel W} δ v :
     constructor
     · intro nvXi
       use []
-      apply witness.nil
-      simp only [modelCanSemImplyForm, evaluatePoint, evaluate]
-      exact nvXi
     · rintro ⟨π, wit⟩
       cases wit
       simp only [modelCanSemImplyForm, evaluatePoint, evaluate] at *
@@ -40,19 +106,21 @@ theorem existsWitnessPath {M : KripkeModel W} δ v :
       intro w v_d_w not_w_
       rw [IH] at not_w_
       clear IH
-      rcases not_w_ with ⟨π, wit⟩
+      rcases not_w_ with ⟨π, w_π_δ_wit⟩
       cases d -- Distinguish cases by the first program `d` in the path `d :: δ`.
       all_goals simp only [relate] at v_d_w
       case atom_prog a =>
-        exact ⟨w :: π, witness.consAtom v_d_w wit⟩
+        exact ⟨w :: π, witness.consAtom v_d_w w_π_δ_wit⟩
       case test φ =>
         rcases v_d_w with ⟨v_is_w, v_φ⟩
         subst v_is_w
         use π
-        apply witness.consEmpty [φ] (by simp [H]) (by simp [modelCanSemImplyList]; exact v_φ) wit
+        exact witness.consEmpty [φ] (by simp [H]) (by simp [modelCanSemImplyList]; exact v_φ) w_π_δ_wit
       -- NEXT: in all remaining cases, use witness.consComp
       -- QUESTION: Do we need IHs/recursion now? What if δ becomes longer in the recursive call?
       case sequence α β =>
+        rcases v_d_w with ⟨u, v_α_u, u_β_w⟩
+
         sorry
       case union α β =>
         sorry
@@ -60,3 +128,4 @@ theorem existsWitnessPath {M : KripkeModel W} δ v :
         sorry
     ·
       sorry
+-/
